avoid overflow of pointer offset

ebpf/Size.v
@@ -6,17 +6,37 @@
 Require Import Coqlib Errors Maps.
 Require Import AST Zbits Integers Floats Values Memory Globalenvs.
 
+Definition is_16_signed (n:Z) :=
+  Z.leb (-(2^15)) n && Z.leb n (2^15 - 1).
+
+Definition is_int (n:Z) :=
+  Z.leb Int.min_signed n && Z.leb n Int.max_signed.
+
 Module Ptrofs.
 
   Definition is_16_signed (p:ptrofs) :=
-    let i := Ptrofs.signed p in
-    Z.leb (-(2^15)) i && Z.leb i (2^15 - 1).
+    is_16_signed (Ptrofs.signed p).
 
   Definition is_int (n:ptrofs) :=
     if negb Archi.ptr64 then true
-    else
-      let i := Ptrofs.signed n in
-      Z.leb Int.min_signed i && Z.leb i Int.max_signed.
-
+    else is_int (Ptrofs.signed n).
 
 End Ptrofs.
+
+Module Int64.
+
+  Definition is_16_signed (p:int64) :=
+    is_16_signed (Int64.signed p).
+
+  Definition is_int (n:int64) :=
+    if negb Archi.ptr64 then true
+    else is_int (Int64.signed n).
+
+End Int64.
+
+Module Int.
+
+  Definition is_16_signed (p:int) :=
+    is_16_signed (Int.signed p).
+
+End Int.
